@prefix products: <http://recipes-project.com/products#> .
@base <http://recipes-project.com/recipe_product_categories> .
@prefix dbc:    <http://dbpedia.org/page/> .
@prefix skos: <http://www.w3.org/2004/02/skos/core#> .
@prefix rdf: <http://www.w3.org/1999/02/22-rdf-syntax-ns#> .
@prefix rdfs: <http://www.w3.org/2000/01/rdf-schema#> .
@prefix : <http://recipes-project.com/schema#> .

# Concepts related to recipe product categories #

<Food> a skos:Concept;
    skos:prefLabel "Food"@en, "Nourriture"@fr;
    skos:exactMatch dbc:Category:Foods;
    skos:broader dbc:Category:Food_and_drink;
    skos:narrower dbc:Category:Types_of_food;
    skos:definition "The substance is ingested by an organism and assimilated by the organism's cells in an effort to produce energy, maintain life, or stimulate growth"@en .

<CerealGrains> a :ProductCategory, skos:Concept;
    skos:prefLabel "Cereals and Grains"@en, "Céréales et graines"@fr;
    skos:narrower dbc:Grains;
    skos:narrower dbc:Cereals;
    skos:related dbc:Pseudocereals .

<FruitsVegetables> a :ProductCategory, skos:Concept;
    skos:prefLabel "Fruits and Vegetables"@en, "Fruits et légumes"@fr;
    skos:member <Fruits>, <Vegetables> .

<Fruits> a :ProductCategory, skos:Concept;
    skos:prefLabel "Fruits"@en, "Fruits"@fr;
    skos:definition "fruit normally means the seed-associated fleshy structures (or produce) of plants that typically are sweet or sour and edible in the raw state, such as apples, bananas, grapes, lemons, oranges, and strawberries"@en,
                    "un fruit est un aliment végétal, à la saveur sucrée, généralement consommé cru"@fr ;
    skos:exactMatch dbc:Category:Fruits;
    skos:relatedMatch dbc:Category:Edible_Fruits .

<Vegetables> a :ProductCategory, skos:Concept;
    skos:prefLabel "Vegetables"@en, "Légumes"@fr;
    skos:definition "Vegetables are parts of plants that are consumed by humans or other animals as food"@en,
                    "Un légume est la plante ou la partie d'une plante comestible d'une espèce potagère"@fr .

<LegumesMeatPoultryFishEggs> a skos:Collection;
    skos:prefLabel "Legumes, Meat, Poultry, Fish, and Eggs"@en, "Légumineuses, Viande, Volaille, Poisson et Oeufs"@fr;
    skos:member <Legumes>, <Meat>, <Poultry>, <Fish>, <Eggs> .

<Legumes> a :ProductCategory, skos:Concept;
    skos:prefLabel "Legumes"@en, "Légumineuses"@fr;
    skos:altLabel "Légumes secs"@fr;
    skos:definition "Les légumes secs, appelés aussi légumineuses à grosses graines, sont des plantes issues exclusivement de la famille des Fabacées"@fr,
                    "A legume is a plant in the family Fabaceae (or Leguminosae)"@en .

<Meat> a :ProductCategory, skos:Concept;
    skos:prefLabel "Meat"@en, "Viande"@fr;
    skos:exactMatch dbc:Category:Meat ;
    skos:related dbc:Poultry, dbc:Sausages, dbc:Charcuterie .

<Poultry> a :ProductCategory, skos:Concept;
    skos:prefLabel "Poultry"@en, "Volaille"@fr;
    skos:exactMatch dbc:Category:Poultry ;
    skos:related dbc:Meat .

<Fish> a :ProductCategory, skos:Concept;
    skos:prefLabel "Fish"@en, "Poisson"@fr;
    skos:exactMatch dbc:Category:Fish .

<Eggs> a :ProductCategory, skos:Concept;
    skos:prefLabel "Eggs"@en, "Oeufs"@fr;
    skos:exactMatch dbc:Category:Eggs ;
    skos:broader <Poultry> .

<MilkDairy> a skos:Collection;
    skos:prefLabel "Milk and Dairy"@en, "Lait et Produits laitiers"@fr;
    skos:member <Milk>, <Dairy> .

<Milk> a :ProductCategory, skos:Concept;
    skos:prefLabel "Milk"@en, "Lait"@fr ;
    skos:exactMatch dbc:Category:Milk .

<Dairy> a :ProductCategory, skos:Concept;
    skos:prefLabel "Dairy"@en, "Produits Laitiers"@fr;
    skos:exactMatch dbc:Category:Dairy;
    skos:closeMatch dbc:Category:Dairy_Products ;
    skos:related dbc:Category:List_of_dairy_products .
    



